\documentclass[a4paper,12pt]{report}
\usepackage[utf8]{inputenc}
\usepackage[T1]{fontenc}
\usepackage[french]{babel}
\usepackage{amsfonts}
\usepackage{amsmath}

\begin{document}
	
		\begin{equation}
		   (\sum_{k=0}^{n}(a_{k}))(\sum_{k=0}^{n}(b_{k}))=a_{1}(\sum_{k=0}^{n}(b_{k}))+...+a_{n}(\sum_{k=0}^{n}(b_{k})) =\sum_{j=0}^{n}a_{j}(\sum_{k=0}^{n}(b_{k}))
		\end{equation}
	
		\begin{equation}
			    \prod_{k=m}^{n}\lambda a_{k} = \lambda^{n - m+1}(\prod_{k=m}^{n}a_{k})
			\end{equation}
	
	
	\begin{equation}
		f :\mathbb{R} \to \mathbb{R}  \\
		\quad \quad  x \mapsto f(x)\left \{
		\begin{array}{r c l}
			sin(\frac{1}{x}), si x \neq 0 \\
			k ,  si x =0\\
		\end{array}
		\right .
	\end{equation}
	
	\begin{equation}
		\lvert\frac{f(z) -f(z_{0})}{z - z_{0}}-f'(z_{0})\rvert < \in
	\end{equation}
	
		\begin{equation}
		    \Delta P(x,y) = \frac{\partial^{2} P}{\partial x^{2}}(x,y) +\frac{\partial^{2} P}{\partial y^{2}}(x,y) = 2 - 2= 0
		\end{equation}
	
		\begin{eqnarray}
			    \lim_{x \to 1}  \frac {f(x)-f(1)}{x- 1} & = & \lim_{x \to 1} \frac {\sqrt{x}- 1}{x- 1} \\
		    & = & \lim_{x \to 0} \frac {\sqrt{x}- 1}{(\sqrt{x}+ 1)(\sqrt{x}- 1)} \\
			    & = & \lim_{x \to 0}\frac {1}{\sqrt{x}+ 1} \\
		    & = & \frac{1}{2} \\
		\end{eqnarray}
	
	
	
\end{document}